Experiments/Test_Suite_Calculation_Refined.thy
@@ -585,7 +585,8 @@ next
     case False
     then have "?v2 = set (paths (from_list (RBT_Set2.keys t)))" using Some by auto
     moreover have "?v1 = set (paths (from_list (RBT_Set2.keys t)))"
-      using False unfolding RBT_set_conv_keys[OF *, of t] remove_proper_prefixes_code_trie by (cases "RBT_Set2.keys t"; auto)
+      using False unfolding RBT_set_conv_keys[OF *, of t] remove_proper_prefixes_code_trie 
+      by (cases "RBT_Set2.keys t"; auto)
     ultimately show ?thesis by simp
   qed
 qed
